# matrices-19005081

Primera parte:
1.1

![imagen 1](https://github.com/user-attachments/assets/1c48887c-4352-481c-9853-00eb5fa57e64)

A+B = [ 2+1  3+5] 
      [4+0  1+2]
      
A+B =        [3  8]
             [4  3]
![imagen2](https://github.com/user-attachments/assets/c351f368-b93d-4bc0-a747-2c91563baeb1)

A+B =      [1+9  2+8  3+7]
	         [4+6  5+5  6+4]
	         [7+3  8+2  9+1]

A+B =  [10  10  10]
	     [10  10  10]
	     [10  10  10]

â€ƒ
1.3 Demuestre que (A + B) + C = A + (B + C):

![imagen3](https://github.com/user-attachments/assets/c7b5187e-4848-4d27-9457-a95f000348e0)

Calcular (A+B) +C 
A+B  =  [1+4    0+(-1) ]         =     [5     -1]
	      [-2+2    3+0    ]		           [0      3]
       
Se suma (A+B) +C
(A+B) +C =   [5   -1]        +      [3      2]        = [5+3      -1+2  ]
	           [0    3] 	            [-1     1]	        [0+(-1)    3+1]

            (A+B) +C = [8     1]
	                     [ -1  4]	



